* hopefully done
some refactoring, some renaming

src/v1-current/Amendment.v
@@ -1,5 +1,7 @@
 Require Import EPP.
 
+(** * Amendment *)
+
 Section Amendment.
 
 Variable Sig : Signature.
@@ -19,210 +21,16 @@ Notation Sig' := (Sig' Sig).
 Local Ltac eq_elim t t' H := case (eq_dec t t'); intro H;
   [ rewrite <- H in *; clear t' H | idtac].
 
-Open Scope CC_scope.
+Local Ltac sup := rewrite set_union_iff; auto.
 
-(** Move me. *)
-Lemma update_idempotent : forall (s:(State Pid Var Value)) p x,
-  s[[p,x=>s p x]] [==] s.
-Proof.
-red; red; intros.
-unfold update, Lupdate. case_eq (p =? p0).
-2: intros; ESEr.
-intro. rewrite eqb_eq in H; rewrite <- H; clear p0 H.
-case_eq (x =? x0).
-2: intros; ESEr.
-intro. rewrite eqb_eq in H; rewrite <- H; auto.
-Qed.
-
-Notation Forget := (@forget Pid Value Var RecVar).
-
-Lemma disjoint_p_rl_eq : forall p t t', Forget t = Forget t' ->
-  disjoint_p_rl p t -> disjoint_p_rl p t'.
-Proof.
-intros. induction t, t'; inversion H; auto.
-all: rewrite H2 in *; auto.
-all: rewrite H3, H4 in *; auto.
-Qed.
-
-Lemma disjoint_eta_rl_eq : forall eta t t', Forget t = Forget t' ->
-  disjoint_eta_rl _ eta t -> disjoint_eta_rl _ eta t'.
-Proof.
-intros. induction eta, t, t'; inversion H; auto.
-all: rewrite H2 in *; auto.
-all: rewrite H3, H4 in *; auto.
-Qed.
-
-Open Scope SP_scope.
-
-Lemma epp_EmptyNet' : forall Xs ps P HP N, Program_WF Sig Xs P ->
-  N (==) nnil -> N (>>) Net (epp Xs ps P HP) -> Main P = CC.End.
-Proof.
-intros. rename H into HWF, H1 into HN, H0 into HN'.
-induction P as (D,C).
-assert (projectable_C D C ps) as HC.
-1: inversion HP; auto.
-generalize (epp_C_char _ _ _ _ _ HP HC); intro.
-destruct C; auto. induction e.
-1,2: rename t0 into p. 3: rename t into p.
-1,2,3: specialize (HN p); rewrite HN', H in HN; simpl in HN.
-- rewrite epp_C_Com_p with (HC':=projectable_C_inv_Com _ _ _ _ _ _ _ _ _ HC) in HN.
-  inversion HN; auto.
-  inversion HP. inversion_clear H1. inversion_clear H3.
-  apply H1; simpl. rewrite set_union_iff; simpl; auto.
-- rewrite epp_C_Sel_p with (HC':=projectable_C_inv_Sel _ _ _ _ _ _ _ _ HC) in HN.
-  inversion HN; auto.
-  inversion HP. inversion_clear H1. inversion_clear H3.
-  apply H1; simpl. rewrite set_union_iff; simpl; auto.
-- rewrite epp_C_Cond_p with (HC1:=projectable_C_inv_Then _ _ _ _ _ _ _ HC)
-        (HC2:=projectable_C_inv_Else _ _ _ _ _ _ _ HC) in HN.
-  inversion HN; auto.
-  inversion HP. inversion_clear H1. inversion_clear H3.
-  apply H1; simpl. repeat rewrite set_union_iff; simpl; auto.
-- generalize (Program_WF_Main_within_Xs _ _ _ HWF); intro.
-  simpl in H0.
-  generalize (Program_WF_Vars _ _ _ HWF t H0); intros.
-  case_eq (Vars (D,CC.Call t) t); intro. tauto.
-  rename t0 into p. intros. clear H1.
-  specialize (HN p). rewrite HN', H, epp_C_Call in HN.
-  3: { unfold Vars in H2. simpl in H2.
-       rewrite H2; simpl; auto. }
-  2: { inversion_clear HP. destroy H3.
-       apply H6 with t; simpl; auto.
-       unfold Vars in H2. simpl in H2.
-       rewrite H2; simpl; auto. }
-  inversion HN; auto.
-- apply Program_WF_Main, Choreography_WF_no_empty_ann in HWF.
-  induction HWF as [H2 H2'].
-  case_eq l; intro. tauto.
-  rename t0 into p. intros.
-  specialize (HN p). rewrite HN', H, epp_C_RT_Call in HN.
-  3: rewrite H0; simpl; auto.
-  inversion HN; auto.
-  apply HP; simpl. rewrite set_union_iff, H0; simpl; auto.
-Qed.
-
-Lemma epp_EmptyNet : forall Xs ps P HP, Program_WF Sig Xs P ->
-  nnil (>>) Net (epp Xs ps P HP) -> Main P = CC.End.
-Proof.
-intros.
-apply epp_EmptyNet' with (N:=nnil) (HP:=HP); auto.
-apply Network_eq_refl.
-Qed.
-
-Close Scope SP_scope.
-
-(** For characterising traces created by amendment. *)
-
-Inductive sel_subtrace : list (TransitionLabel Pid Value) -> list (TransitionLabel Pid Value) -> Prop :=
-| ss_base l l' : Permutation l l' -> sel_subtrace l l'
-(* | ss_cons t l l' l'' : sel_subtrace l l' -> Permutation (t::l') l'' -> sel_subtrace l l'' *)
-| ss_extra p q la l l' l'' : sel_subtrace l l' -> Permutation (TL_Sel p q la::l') l'' -> sel_subtrace l l''.
-
-Lemma sel_subtrace_refl : forall ts, sel_subtrace ts ts.
-Proof. constructor. auto. Qed.
-
-Lemma sel_subtrace_cons : forall t ts ts',
-  sel_subtrace ts ts' -> sel_subtrace (t::ts) (t::ts').
-Proof.
-intros. induction H.
-- apply ss_base; auto.
-- apply ss_extra with p q la (t::l'); auto.
-  eapply Permutation_trans. apply perm_swap. auto.
-Qed.
-
-Lemma sel_subtrace_extra : forall p q l ts ts',
-  sel_subtrace ts ts' -> sel_subtrace ts (TL_Sel p q l::ts').
-Proof.
-intros.
-apply ss_extra with p q l ts'; auto.
-Qed.
-
-Lemma sel_subtrace_app : forall ts ts' ts'',
-  sel_subtrace ts' ts'' -> sel_subtrace (ts++ts') (ts++ts'').
-Proof.
-induction ts; intros; auto.
-apply sel_subtrace_cons; auto.
-Qed.
-
-Lemma sel_subtrace_perm' : forall ts ts' ts'',
-  sel_subtrace ts ts' -> Permutation ts' ts'' -> sel_subtrace ts ts''.
-Proof.
-intros. induction H.
-- apply ss_base. eapply perm_trans; eauto.
-- apply ss_extra with p q la l'; auto.
-  eapply Permutation_trans; eauto.
-Qed.
-
-Lemma sel_subtrace_perm : forall ts ts' ts'',
-  sel_subtrace ts ts' -> Permutation ts'' ts -> sel_subtrace ts'' ts'.
-Proof.
-intros. induction H.
-- apply ss_base. eapply perm_trans; eauto.
-- apply ss_extra with p q la l'; auto.
-Qed.
-
-Lemma sel_subtrace_trans : forall ts ts' ts'',
-  sel_subtrace ts ts' -> sel_subtrace ts' ts'' -> sel_subtrace ts ts''.
-Proof.
-intros. induction H0.
-- apply sel_subtrace_perm' with l; auto.
-- apply ss_extra with p q la l'; auto.
-Qed.
-
-Lemma sel_subtrace_swap : forall t t' ts ts',
-  sel_subtrace ts (t :: ts') -> sel_subtrace (t' :: ts) (t :: t' :: ts').
-Proof.
-intros.
-eapply sel_subtrace_perm'.
-2: apply perm_swap.
-apply sel_subtrace_cons; auto.
-Qed.
-
-Lemma sel_subtrace_perm_extra : forall t t' ts ts' p q l,
-  sel_subtrace ts (t :: ts') -> sel_subtrace (t' :: ts) (t :: t' :: (TL_Sel p q l) :: ts').
-Proof.
-intros.
-eapply sel_subtrace_trans. 2: apply sel_subtrace_swap.
-apply sel_subtrace_cons; eauto.
-apply sel_subtrace_cons, sel_subtrace_extra.
-apply sel_subtrace_refl.
-Qed.
-
-Lemma sel_subtrace_app' : forall t ts ts' ts'',
-  sel_subtrace ts (t::ts') -> sel_subtrace (ts''++ts) (t::ts''++ts').
-Proof.
-intros.
-apply sel_subtrace_perm' with (ts''++t::ts').
-apply sel_subtrace_app; auto.
-apply Permutation_sym, Permutation_middle.
-Qed.
-
-Lemma sel_subtrace_app'' : forall t ts ts' ts'',
-  sel_subtrace ts (ts' ++ ts'') -> sel_subtrace (t :: ts) (ts' ++ t :: ts'').
-Proof.
-intros.
-eapply sel_subtrace_trans.
-apply sel_subtrace_cons; eauto.
-constructor. apply Permutation_middle.
-Qed.
-
-Lemma sel_subtrace_app_both : forall ts1 ts1' ts2 ts2',
-  sel_subtrace ts1 ts1' -> sel_subtrace ts2 ts2' -> sel_subtrace (ts1++ts2) (ts1'++ts2').
-Proof.
-intros.
-eapply sel_subtrace_trans.
-apply sel_subtrace_app; eauto.
-eapply sel_subtrace_perm.
-2: apply Permutation_app_comm.
-eapply sel_subtrace_perm'.
-2: apply Permutation_app_comm.
-apply sel_subtrace_app; auto.
-Qed.
+(** ** Definitions *)
 
 Section Amend.
 
 Variable Defs:DefSet Sig.
 Variable a:Ann.
+
+(** The unprojectable processes at a conditional. *)
 
 Fixpoint up_list p b ps C1 C2 : list Pid :=
   match ps with
@@ -233,21 +41,30 @@ Fixpoint up_list p b ps C1 C2 : list Pid :=
                 then ps'' else (r :: ps'')
   end.
 
+(** Add selections from p to all processes in ps. *)
+
 Fixpoint add_sels p l ps C : Choreography Sig :=
   match ps with
   | nil => C
   | r :: ps' => p --> r[l]@a;; add_sels p l ps' C
   end.
 
+Open Scope CC_scope.
+
+(** Amending a choreography. *)
+
 Fixpoint amend (ps:list Pid) (C:Choreography Sig) :=
 match C with
 | eta@a';; C' => eta@a';; (amend ps C')
 | If p ?? b Then C1 Else C2 =>
     let l := up_list p b ps (amend ps C1) (amend ps C2) in
-    If p ?? b Then (add_sels p left l (amend ps C1)) Else (add_sels p right l (amend ps C2))
+    If p ?? b Then (add_sels p left l (amend ps C1))
+              Else (add_sels p right l (amend ps C2))
 | RT_Call X l C' => RT_Call X l (amend ps C')
 | _ => C
 end.
+
+(** Generalization to a set of procedure definitions. *)
 
 Definition amend_D ps : DefSet Sig :=
   fun X => (fst (Defs X), amend ps (snd (Defs X))).
@@ -258,8 +75,6 @@ Lemma up_list_If : forall p b r ps C1 C2,
   { up_list p b (r::ps) C1 C2 = up_list p b ps C1 C2 }
   + { up_list p b (r::ps) C1 C2 = r :: up_list p b ps C1 C2 }.
 Proof. intros; simpl. elim (r =? p); auto. elim projectable_B_dec; auto. Qed.
-
-(** Amendment preserves well-formedness. *)
 
 Lemma not_In_up_list : forall p b ps C1 C2,
   ~In p (up_list p b ps C1 C2).
@@ -272,6 +87,8 @@ inversion_clear H0; auto.
 rewrite eqb_neq in H; auto.
 apply (IHps _ _ H1).
 Qed.
+
+(** General properties of [up_list] *)
 
 Lemma not_In_up_list' : forall p b ps C1 C2 r, p <> r -> In r ps ->
   ~In r (up_list p b ps C1 C2) ->
@@ -289,6 +106,89 @@ inversion_clear H0.
   intro. apply IHps; auto.
   intro; apply H1; simpl; auto.
 Qed.
+
+(** Amendment does not add new process names to a choreography. *)
+
+Lemma up_list_incl : forall p b ps C1 C2, up_list p b ps C1 C2 [C] ps.
+Proof.
+red; intros. induction ps; simpl; auto.
+revert H; simpl. elim eqb; auto.
+elim projectable_B_dec; auto.
+simpl; intros. inversion_clear H; auto.
+Qed.
+
+Lemma up_list_incl_C : forall p b ps C1 C2,
+  up_list p b ps C1 C2 [C] (CCC_pn C1 (Names Defs) [U] CCC_pn C2 (Names Defs)).
+Proof.
+red; intros. induction ps; simpl; auto. inversion H.
+generalize H; simpl.
+case_eq (a0 =? p); intro; auto.
+elim projectable_B_dec; intros; auto.
+elim (In_dec (@eq_dec Pid) z (up_list p b ps C1 C2)); auto.
+intro. inversion_clear H1; auto.
+rewrite H2 in *; clear a H2.
+elim (In_dec (@eq_dec Pid) z (CCC_pn C1 (Names Defs) [U] CCC_pn C2 (Names Defs))); auto.
+intro. elim b0.
+exists (End _). apply bproj_not_In; auto.
+simpl. repeat sup.
+intro; apply b2. repeat sup. 
+induction H1 as [ [H1 | H1] | H1]; auto.
+rewrite eqb_neq in H0. simpl in H1.
+inversion_clear H1; exfalso; auto.
+Qed.
+
+Lemma add_sels_CCC_pn_C : forall ps p l C f,
+  CCC_pn C f [C] CCC_pn (add_sels p l ps C) f.
+Proof. red; intros. induction ps; simpl; auto. sup. Qed.
+
+Lemma add_sels_CCC_pn_ps : forall ps p l C f,
+  ps [C] CCC_pn (add_sels p l ps C) f.
+Proof.
+red; intros.
+induction ps, H.
+all: simpl; sup. rewrite H; simpl; auto.
+Qed.
+
+Lemma add_sels_CCC_pn : forall ps p l C f,
+  CCC_pn (add_sels p l ps C) f [C] (p :: CCC_pn C f [U] ps).
+Proof.
+intros; induction ps; simpl; auto.
+red; simpl; auto.
+red; red in IHps; intros.
+simpl; rewrite set_add_iff.
+rewrite set_union_iff in H.
+induction H as [ [H | [H | H] ] | H]; auto.
+inversion H. elim (IHps z); auto.
+Qed.
+
+Lemma amend_CCC_pn_C : forall ps f C, CCC_pn C f [C] CCC_pn (amend ps C) f.
+Proof.
+red; intros. induction C; simpl; auto.
+all: sup.
++ induction e; simpl in H; rewrite set_union_iff in H; tauto.
++ simpl in H. repeat rewrite set_union_iff in H.
+  induction H as [ [H | H] | H]; sup.
+  1: left; right. 2: right.
+  all: apply add_sels_CCC_pn_C; auto.
++ simpl in H. rewrite set_union_iff in H; tauto.
+Qed.
+
+Lemma amend_CCC_pn_incl : forall ps C,
+  CCC_pn (amend ps C) (Names Defs) [C] CCC_pn C (Names Defs).
+Proof.
+red; intros. induction C. induction e.
+all: simpl; auto.
+all: simpl in H; repeat rewrite set_union_iff in H.
+all: inversion_clear H; repeat sup.
+inversion_clear H0; auto.
+2: rename H0 into H.
+all: apply add_sels_CCC_pn in H.
+all: inversion_clear H. 1,3: rewrite H0; simpl; auto.
+all: rewrite set_union_iff in H0; inversion_clear H0; auto.
+all: apply up_list_incl_C in H; rewrite set_union_iff in H; tauto.
+Qed.
+
+(** Amendment preserves well-formedness. *)
 
 Lemma add_sels_no_self_comm : forall p l ps C, ~In p ps ->
   no_self_comm _ C -> no_self_comm _ (add_sels p l ps C).
@@ -333,7 +233,8 @@ induction C; auto; intros.
 + destroy H; split; auto.
 Qed.
 
-Lemma amend_Choreography_WF : forall ps C, Choreography_WF C -> Choreography_WF (amend ps C).
+Lemma amend_Choreography_WF : forall ps C,
+  Choreography_WF C -> Choreography_WF (amend ps C).
 Proof.
 intros.
 destroy H; split.
@@ -354,12 +255,12 @@ induction C; auto; intros.
 + destroy H. split; auto.
 Qed.
 
-Lemma add_sels_consistent : forall p l ps C,
-  consistent _ (Vars (Defs,C)) C -> consistent _ (Vars (amend_D ps,add_sels p l ps C)) (add_sels p l ps C).
+Lemma add_sels_consistent : forall p l ps C, consistent _ (Vars (Defs,C)) C ->
+  consistent _ (Vars (amend_D ps,add_sels p l ps C)) (add_sels p l ps C).
 Proof. induction ps; auto. Qed.
 
-Lemma amend_consistent : forall ps C,
-  consistent _ (Vars (Defs,C)) C -> consistent _ (Vars (amend_D ps,amend ps C)) (amend ps C).
+Lemma amend_consistent : forall ps C, consistent _ (Vars (Defs,C)) C ->
+  consistent _ (Vars (amend_D ps,amend ps C)) (amend ps C).
 Proof.
 induction C; auto; intros.
 + inversion_clear H.
@@ -383,24 +284,164 @@ destroy H. split. 2: split. 3: split.
   - apply amend_within_Xs; auto.
 Qed.
 
-(** Completeness *)
+(** ** Selection expansion up to permutation
+  This relation is used for characterising traces created by amendment. *)
+
+Inductive sel_exp :
+  list (TransitionLabel Pid Value) -> list (TransitionLabel Pid Value) -> Prop :=
+| se_base l l' : Permutation l l' -> sel_exp l l'
+| se_extra p q la l l' l'' : sel_exp l l' ->
+                             Permutation (TL_Sel p q la::l') l'' -> sel_exp l l''.
+
+Lemma sel_exp_refl : forall ts, sel_exp ts ts.
+Proof. constructor. auto. Qed.
+
+Lemma sel_exp_cons : forall t ts ts',
+  sel_exp ts ts' -> sel_exp (t::ts) (t::ts').
+Proof.
+intros. induction H.
+- apply se_base; auto.
+- apply se_extra with p q la (t::l'); auto.
+  eapply Permutation_trans. apply perm_swap. auto.
+Qed.
+
+Lemma sel_exp_extra : forall p q l ts ts',
+  sel_exp ts ts' -> sel_exp ts (TL_Sel p q l::ts').
+Proof.
+intros.
+apply se_extra with p q l ts'; auto.
+Qed.
+
+Lemma sel_exp_app : forall ts ts' ts'',
+  sel_exp ts' ts'' -> sel_exp (ts++ts') (ts++ts'').
+Proof.
+induction ts; intros; auto.
+apply sel_exp_cons; auto.
+Qed.
+
+Lemma sel_exp_perm' : forall ts ts' ts'',
+  sel_exp ts ts' -> Permutation ts' ts'' -> sel_exp ts ts''.
+Proof.
+intros. induction H.
+- apply se_base. eapply perm_trans; eauto.
+- apply se_extra with p q la l'; auto.
+  eapply Permutation_trans; eauto.
+Qed.
+
+Lemma sel_exp_perm : forall ts ts' ts'',
+  sel_exp ts ts' -> Permutation ts'' ts -> sel_exp ts'' ts'.
+Proof.
+intros. induction H.
+- apply se_base. eapply perm_trans; eauto.
+- apply se_extra with p q la l'; auto.
+Qed.
+
+Lemma sel_exp_trans : forall ts ts' ts'',
+  sel_exp ts ts' -> sel_exp ts' ts'' -> sel_exp ts ts''.
+Proof.
+intros. induction H0.
+- apply sel_exp_perm' with l; auto.
+- apply se_extra with p q la l'; auto.
+Qed.
+
+Lemma sel_exp_swap : forall t t' ts ts',
+  sel_exp ts (t :: ts') -> sel_exp (t' :: ts) (t :: t' :: ts').
+Proof.
+intros.
+eapply sel_exp_perm'.
+2: apply perm_swap.
+apply sel_exp_cons; auto.
+Qed.
+
+Lemma sel_exp_perm_extra : forall t t' ts ts' p q l,
+  sel_exp ts (t :: ts') -> sel_exp (t' :: ts) (t :: t' :: (TL_Sel p q l) :: ts').
+Proof.
+intros.
+eapply sel_exp_trans. 2: apply sel_exp_swap.
+apply sel_exp_cons; eauto.
+apply sel_exp_cons, sel_exp_extra.
+apply sel_exp_refl.
+Qed.
+
+Lemma sel_exp_app' : forall t ts ts' ts'',
+  sel_exp ts (t::ts') -> sel_exp (ts''++ts) (t::ts''++ts').
+Proof.
+intros.
+apply sel_exp_perm' with (ts''++t::ts').
+apply sel_exp_app; auto.
+apply Permutation_sym, Permutation_middle.
+Qed.
+
+Lemma sel_exp_app'' : forall t ts ts' ts'',
+  sel_exp ts (ts' ++ ts'') -> sel_exp (t :: ts) (ts' ++ t :: ts'').
+Proof.
+intros.
+eapply sel_exp_trans.
+apply sel_exp_cons; eauto.
+constructor. apply Permutation_middle.
+Qed.
+
+Lemma sel_exp_app_both : forall ts1 ts1' ts2 ts2',
+  sel_exp ts1 ts1' -> sel_exp ts2 ts2' -> sel_exp (ts1++ts2) (ts1'++ts2').
+Proof.
+intros.
+eapply sel_exp_trans.
+apply sel_exp_app; eauto.
+eapply sel_exp_perm.
+2: apply Permutation_app_comm.
+eapply sel_exp_perm'.
+2: apply Permutation_app_comm.
+apply sel_exp_app; auto.
+Qed.
+
+(** Selections added by [add_sels] can be removed by a trace containing only selections. *)
 
 Lemma add_sels_reduce : forall D p l ps C s,
-  exists tl, sel_subtrace nil tl /\
+  exists tl, sel_exp nil tl /\
     (D,add_sels p l ps C,s) --[tl]-->* (D,C,s).
 Proof.
 induction ps; simpl; intros.
-+ exists nil. split. apply sel_subtrace_refl. apply CCT_Refl.
++ exists nil. split. apply sel_exp_refl. apply CCT_Refl.
 + induction (IHps C s) as [tl [Hsub Htl] ].
   exists (@forget Pid Value Var RecVar (RL_Sel p a0 l)::tl).
-  split. apply sel_subtrace_extra; auto.
+  split. apply sel_exp_extra; auto.
   econstructor; eauto. repeat constructor; auto.
 Qed.
+
+(** If we added different selections to two choreographies, then
+  any moves they both can perform must have been possible already. *)
+
+Lemma add_sels_reduce_both : forall p ps C1 C2 s tl D C1' C2' s',
+  <<add_sels p left ps C1,s>> --[tl,D]--> <<C1',s'>> ->
+  <<add_sels p right ps C2,s>> --[tl,D]--> <<C2',s'>> ->
+  exists C1'' C2'', <<C1,s>> --[tl,D]--> <<C1'',s'>>
+    /\ <<C2,s>> --[tl,D]--> <<C2'',s'>>
+    /\ C1' = add_sels p left ps C1'' /\ C2' = add_sels p right ps C2''.
+Proof.
+induction ps; simpl; intros.
++ exists C1', C2'; auto.
++ inversion H; inversion H0.
+  1: rewrite <- H17 in H7; inversion H7.
+  1: rewrite <- H7 in H18. simpl in H18. tauto.
+  1: rewrite <- H16 in H8. simpl in H8. tauto.
+  elim (IHps _ _ _ _ _ _ _ _ H9 H18).
+  intros C1'' (C2'',(HC1,(HC2,(HC1',HC2')))).
+  repeat eexists; repeat split; eauto.
+  rewrite HC1'; auto.
+  rewrite HC2'; auto.
+Qed.
+
+(** Miscellaneous. *)
+
+Lemma amend_eq_End : forall ps C, amend ps C = CC.End -> C = CC.End.
+Proof. induction C; simpl; auto; discriminate. Qed.
+
+(** ** Completeness *)
 
 Lemma amend_complete_1 : forall ps C s tl C' s', Choreography_WF C ->
   (Defs,C,s) --[tl]--> (Defs,C',s') ->
   exists tl' tlI tlF C'' s'',
-       sel_subtrace tl' (tlI++tlF)
+       sel_exp tl' (tlI++tlF)
     /\ (Defs,C',s') --[tl']-->* (Defs,C'',s'')
     /\ (amend_D ps,amend ps C,s) --[tlI ++ tl::tlF]-->* (amend_D ps,amend ps C'',s'').
 Proof.
@@ -409,7 +450,7 @@ Local Ltac IHElim IHC HC H tl' tlI CI sI tl0 C0 s0 tlF CF sF H1 H2 H3 H4 H5 H6 :
     [tl' [tlI [CI [sI [tl0 [C0 [s0 [tlF [CF [sF [H1 [H2 [H3 [H4 [H5 H6] ] ] ] ] ] ] ] ] ] ] ] ] ] ]; clear IHC.
 intros. rename H into HC, H0 into H.
 assert (exists tl' tlI CI sI tl0 C0 s0 tlF CF sF,
-       sel_subtrace tl' (tlI++tlF)
+       sel_exp tl' (tlI++tlF)
     /\ tl = forget tl0
     /\ (Defs,C',s') --[tl']-->* (Defs,CF,sF)
     /\ (amend_D ps,amend ps C,s) --[tlI]-->* (amend_D ps,CI,sI)
@@ -431,7 +472,7 @@ induction C; intros. induction e.
     simpl. exists nil, nil; do 2 eexists.
     exists (RL_Com p v q x), (amend ps C), s'.
     exists nil, C, s'.
-    repeat split; eauto. apply sel_subtrace_refl.
+    repeat split; eauto. apply sel_exp_refl.
     all: constructor; auto; ESEr.
   - (* Delay *)
     rewrite <- H5 in *.
@@ -445,7 +486,7 @@ induction C; intros. induction e.
     exists (forget tlS::tl'). exists (forget tlS::tlI), CI, sI.
     exists tl0, C0, s0. exists tlF, CF, sF.
     repeat split; auto.
-    * apply sel_subtrace_cons; auto.
+    * apply sel_exp_cons; auto.
     * econstructor; eauto. unfold tlS; rewrite Hv.
       repeat constructor; auto.
     * econstructor; eauto. repeat constructor; auto.
@@ -457,7 +498,7 @@ induction C; intros. induction e.
     simpl. exists nil, nil; do 2 eexists.
     exists (RL_Sel p q l), (amend ps C), s'.
     exists nil, C, s'.
-    repeat split; eauto. apply sel_subtrace_refl.
+    repeat split; eauto. apply sel_exp_refl.
     all: constructor; eauto; try ESEr.
   - (* Delay *)
     rewrite <- H5 in *.
@@ -468,7 +509,7 @@ induction C; intros. induction e.
     exists (forget tlS::tl'). exists (forget tlS::tlI), CI, sI.
     exists tl0, C0, s0. exists tlF, CF, sF.
     repeat split; auto.
-    * apply sel_subtrace_cons; auto.
+    * apply sel_exp_cons; auto.
     * econstructor; eauto. repeat constructor; auto.
     * econstructor; eauto. repeat constructor; auto.
 + rename t into p, t0 into b.
@@ -507,14 +548,14 @@ induction C; intros. induction e.
       set (tl0 := @RL_Cond Pid Value Var RecVar p).
       elim (add_sels_reduce (amend_D ps) p left (up_list p b ps (amend ps C1) (amend ps C2)) (amend ps C1) s).
       intros t1 (Ht1,Ht1').
-      exists (Forget tl0::tl'1).
-      exists (Forget tl0::t1++tl1I), C1I, s1I.
+      exists (Forget _ tl0::tl'1).
+      exists (Forget _ tl0::t1++tl1I), C1I, s1I.
       exists tl01, C01, s01.
       exists tl1F, C1F, s1F.
       repeat split; auto.
-      ++ simpl. apply sel_subtrace_cons.
+      ++ simpl. apply sel_exp_cons.
          rewrite <- (app_nil_l tl'1), <- app_assoc.
-         apply sel_subtrace_app_both; auto.
+         apply sel_exp_app_both; auto.
       ++ econstructor; eauto. repeat constructor. rewrite <- Hb; auto.
       ++ econstructor; eauto. 2: eapply CCT_Trans; eauto.
          repeat constructor; auto.
@@ -522,14 +563,14 @@ induction C; intros. induction e.
       set (tl0 := @RL_Cond Pid Value Var RecVar p).
       elim (add_sels_reduce (amend_D ps) p right (up_list p b ps (amend ps C1) (amend ps C2)) (amend ps C2) s).
       intros t1 (Ht1,Ht1').
-      exists (Forget tl0::tl'2).
-      exists (Forget tl0::t1++tl2I), C2I, s2I.
+      exists (Forget _ tl0::tl'2).
+      exists (Forget _ tl0::t1++tl2I), C2I, s2I.
       exists tl02, C02, s02.
       exists tl2F, C2F, s2F.
       repeat split; auto.
-      ++ simpl. apply sel_subtrace_cons.
+      ++ simpl. apply sel_exp_cons.
          rewrite <- (app_nil_l tl'2), <- app_assoc.
-         apply sel_subtrace_app_both; auto.
+         apply sel_exp_app_both; auto.
       ++ econstructor; eauto. repeat constructor. rewrite <- Hb; auto.
       ++ econstructor; eauto. 2: eapply CCT_Trans; eauto.
          repeat constructor; auto.
@@ -540,7 +581,7 @@ induction C; intros. induction e.
     simpl. exists nil, nil; do 2 eexists.
     exists (RL_Call X p), (amend ps (snd (Defs X))), s'.
     exists nil, (snd (Defs X)), s'.
-    repeat split; eauto. apply sel_subtrace_refl.
+    repeat split; eauto. apply sel_exp_refl.
     all: constructor; simpl; eauto; ESEr.
   - (* Call *)
     rewrite <- H5 in *.
@@ -548,7 +589,7 @@ induction C; intros. induction e.
     simpl. exists nil, nil; do 2 eexists.
     exists (RL_Call X p); eexists; exists s'.
     exists nil; eexists; exists s'.
-    repeat split; eauto. apply sel_subtrace_refl.
+    repeat split; eauto. apply sel_exp_refl.
     all: constructor; simpl; eauto; ESEr.
 + rename t into X. inversion H.
   - (* Delay *)
@@ -560,7 +601,7 @@ induction C; intros. induction e.
     exists (tlR++tl'). exists (tlR++tlI), CI, sI.
     exists tl0, C0, s0. exists tlF, CF, sF.
     repeat split; auto.
-    * rewrite <- app_assoc. apply sel_subtrace_app; auto.
+    * rewrite <- app_assoc. apply sel_exp_app; auto.
     * eapply CCT_Trans; eauto.
     * eapply CCT_Trans; eauto.
   - (* Enter *)
@@ -569,7 +610,7 @@ induction C; intros. induction e.
     simpl. exists nil, nil; do 2 eexists.
     exists (RL_Call X p), (RT_Call X (ps0[\]p) (amend ps C)), s'.
     exists nil; eexists; exists s'.
-    repeat split; eauto. apply sel_subtrace_refl.
+    repeat split; eauto. apply sel_exp_refl.
     all: constructor; eauto; ESEr.
   - (* Finish *)
     rewrite <- H6, <- H1 in *.
@@ -577,7 +618,7 @@ induction C; intros. induction e.
     simpl. exists nil, nil; do 2 eexists.
     exists (RL_Call X p), (amend ps C), s'.
     exists nil, C, s'.
-    repeat split; eauto. apply sel_subtrace_refl.
+    repeat split; eauto. apply sel_exp_refl.
     all: constructor; eauto; ESEr.
 + inversion H.
 Qed.
@@ -585,7 +626,7 @@ Qed.
 Lemma amend_complete_1' : forall ps C s tl C' s', Choreography_WF C ->
   (Defs,C,s) --[tl]--> (Defs,C',s') ->
   exists tl' tl'' C'' s'',
-       sel_subtrace (tl::tl') tl''
+       sel_exp (tl::tl') tl''
     /\ (Defs,C',s') --[tl']-->* (Defs,C'',s'')
     /\ (amend_D ps,amend ps C,s) --[tl'']-->* (amend_D ps,amend ps C'',s'').
 Proof.
@@ -593,13 +634,13 @@ intros.
 elim (amend_complete_1 ps C s tl C' s'); auto.
 intros. induction H1 as (tlI,(tlF,(C'',(s'',(H1,(H2,H3)))))).
 do 4 eexists. repeat split; eauto.
-apply sel_subtrace_app''; auto.
+apply sel_exp_app''; auto.
 Qed.
 
 Lemma amend_complete_many : forall ps C s tl C' s' Xs, Program_WF _ Xs (Defs,C) ->
   (Defs,C,s) --[tl]-->* (Defs,C',s') ->
   exists tl' tl'' C'' s'',
-       sel_subtrace (tl++tl') tl''
+       sel_exp (tl++tl') tl''
     /\ (Defs,C',s') --[tl']-->* (Defs,C'',s'')
     /\ (amend_D ps,amend ps C,s) --[tl'']-->* (amend_D ps,amend ps C'',s'').
 Proof.
@@ -629,18 +670,18 @@ induction n; intros.
   intros tl0 [t0 [C0 [s0 [Hsub0 [Htl0 Htl0IF] ] ] ] ].
   induction (diamond_4b _ _ _ _ _ _ _ _ _ H2 Htl0) as [ [D C2] [tl' [tl0' [s2a [s2b [HC' [HC0 [Hs [Hperm [Hlen1 Hlen2] ] ] ] ] ] ] ] ] ].
   generalize (CCP_ToStar_Defs_stable _ _ _ _ _ _ _ _ HC'). intro H'; rewrite <- H' in *; clear D H'.
-  generalize (CCC_To_Program_WF _ _ _ _ _ _ _ H H1). intro HP''.
-  generalize (CCC_ToStar_Program_WF _ _ _ _ _ _ _ HP'' H2). intro HP'.
-  generalize (CCC_ToStar_Program_WF _ _ _ _ _ _ _ HP' HC'). intro HP2.
-  generalize (CCC_ToStar_Program_WF _ _ _ _ _ _ _ HP'' Htl0). intro HP0.
+  generalize (CCP_To_Program_WF _ _ _ _ _ _ _ H H1). intro HP''.
+  generalize (CCP_ToStar_Program_WF _ _ _ _ _ _ _ HP'' H2). intro HP'.
+  generalize (CCP_ToStar_Program_WF _ _ _ _ _ _ _ HP' HC'). intro HP2.
+  generalize (CCP_ToStar_Program_WF _ _ _ _ _ _ _ HP'' Htl0). intro HP0.
   elim (IHn C0 s0 tl0' C2 s2b); auto.
   intros tl1 [t1 [C1 [s1 [Hsub1 [Htl1 Htl1IF] ] ] ] ].
   2: etransitivity; eauto.
   exists (tl' ++ tl1), (t0 ++ t1), C1, s1.
   repeat split.
-  - simpl. eapply sel_subtrace_trans.
-    2: apply sel_subtrace_app_both; eauto.
-    simpl. apply sel_subtrace_cons.
+  - simpl. eapply sel_exp_trans.
+    2: apply sel_exp_app_both; eauto.
+    simpl. apply sel_exp_cons.
     repeat rewrite app_assoc.
     constructor. apply Permutation_app; auto.
   - eapply CCT_Trans; eauto.
@@ -648,33 +689,13 @@ induction n; intros.
   - eapply CCT_Trans; eauto.
 Qed.
 
-(** Soundness *)
-
-Lemma add_sels_reduce_both : forall p ps C1 C2 s tl D C1' C2' s',
-  <<add_sels p left ps C1,s>> --[tl,D]--> <<C1',s'>> ->
-  <<add_sels p right ps C2,s>> --[tl,D]--> <<C2',s'>> ->
-  exists C1'' C2'', <<C1,s>> --[tl,D]--> <<C1'',s'>>
-    /\ <<C2,s>> --[tl,D]--> <<C2'',s'>>
-    /\ C1' = add_sels p left ps C1'' /\ C2' = add_sels p right ps C2''.
-Proof.
-induction ps; simpl; intros.
-+ exists C1', C2'; auto.
-+ inversion H; inversion H0.
-  1: rewrite <- H17 in H7; inversion H7.
-  1: rewrite <- H7 in H18. simpl in H18. tauto.
-  1: rewrite <- H16 in H8. simpl in H8. tauto.
-  elim (IHps _ _ _ _ _ _ _ _ H9 H18).
-  intros C1'' (C2'',(HC1,(HC2,(HC1',HC2')))).
-  repeat eexists; repeat split; eauto.
-  rewrite HC1'; auto.
-  rewrite HC2'; auto.
-Qed.
+(** ** Soundness *)
 
 Lemma amend_sound_1 : forall ps C s tl C' s', Choreography_WF C ->
   (amend_D ps, amend ps C,s) --[tl]--> (amend_D ps,C',s') ->
   exists tl' tl'' C'' s'',
   (amend_D ps,C',s') --[tl']-->* (amend_D ps, amend ps C'',s'')
-  /\ (Defs,C,s) --[tl'']-->* (Defs,C'',s'') /\ sel_subtrace tl'' (tl::tl').
+  /\ (Defs,C,s) --[tl'']-->* (Defs,C'',s'') /\ sel_exp tl'' (tl::tl').
 Proof.
 Local Ltac IHElim' IHC HC H tl' tl'' C'' s'' Htl' Htl'' Hsub :=
    induction (IHC HC _ _ _ H) as [tl' [tl'' [C'' [s'' [Htl' [Htl'' Hsub] ] ] ] ] ]; clear IHC.
@@ -686,10 +707,10 @@ induction C; intros. induction e.
   - (* Com *)
     rewrite <- H7 in *.
     clear s'0 H9 C' H8 t H7 s0 H1 C0 H6 a0 H5 x0 H4 q0 H3 e0 H2 p0 H H0.
-    exists nil, (Forget (RL_Com p v q x) :: nil), C, s'. repeat split.
+    exists nil, (Forget _ (RL_Com p v q x) :: nil), C, s'. repeat split.
     * repeat constructor.
     * econstructor; eauto. 2: apply CCT_Refl. repeat constructor; auto.
-    * apply sel_subtrace_refl.
+    * apply sel_exp_refl.
   - (* Delay *)
     clear s'0 H6 C' H5 t0 H4 s0 H2 C0 H3 ann H1 eta H H0.
     induction H7 as [Hp Hq].
@@ -698,30 +719,30 @@ induction C; intros. induction e.
     1: unfold v. symmetry; eapply CCC_To_disjoint_eval; eauto.
     apply CCC_To_disjoint_update with (p:=q) (v:=v) (x:=x) in H8; auto.
     IHElim' IHC (Choreography_WF_eta _ _ _ _ HC) H8 tl' tl'' C'' s'' Htl' Htl'' Hsub.
-    exists (Forget tlS::tl'), (Forget tlS::tl''), C'', s''.
+    exists (Forget _ tlS::tl'), (Forget _ tlS::tl''), C'', s''.
     repeat split; auto.
     * econstructor; eauto. unfold v; repeat constructor.
     * econstructor; eauto. unfold tlS; rewrite Hv; repeat constructor.
-    * apply sel_subtrace_swap; auto.
+    * apply sel_exp_swap; auto.
 + rename t1 into p, t2 into q, t3 into l, t0 into a'.
   inversion H.
   - (* Sel *)
     rewrite <- H6 in *.
     clear s'0 H8 C' H7 t H6 s0 H1 C0 H5 a0 H4 l0 H3 q0 H2 p0 H H0.
-    exists nil, (Forget (RL_Sel p q l) :: nil), C, s'. repeat split.
+    exists nil, (Forget _ (RL_Sel p q l) :: nil), C, s'. repeat split.
     * repeat constructor.
     * econstructor; eauto. 2: apply CCT_Refl. repeat constructor; auto.
-    * apply sel_subtrace_refl.
+    * apply sel_exp_refl.
   - (* Delay *)
     clear s'0 H6 C' H5 t0 H4 s0 H2 C0 H3 ann H1 eta H H0.
     induction H7 as [Hp Hq].
     IHElim' IHC (Choreography_WF_eta _ _ _ _ HC) H8 tl' tl'' C'' s'' Htl' Htl'' Hsub.
     set (tlS := @RL_Sel Pid Value Var RecVar p q l).
-    exists (Forget tlS::tl'), (Forget tlS::tl''), C'', s''.
+    exists (Forget _ tlS::tl'), (Forget _ tlS::tl''), C'', s''.
     repeat split; auto.
     * econstructor; eauto. repeat constructor.
     * econstructor; eauto. repeat constructor.
-    * apply sel_subtrace_swap; auto.
+    * apply sel_exp_swap; auto.
 + rename t0 into p, t1 into b.
   inversion H.
   - (* Then *)
@@ -729,17 +750,17 @@ induction C; intros. induction e.
     clear s'0 H7 C' H6 t H5 s0 H2 C3 H4 C0 H3 b0 H1 p0 H0.
     elim (add_sels_reduce (amend_D ps) p left (up_list p b ps (amend ps C1) (amend ps C2)) (amend ps C1) s').
     intros t1 (Ht1,Ht1').
-    exists t1, (Forget (RL_Cond p)::nil), C1, s'. repeat split; auto.
+    exists t1, (Forget _ (RL_Cond p)::nil), C1, s'. repeat split; auto.
     * econstructor. 2: apply CCT_Refl. repeat constructor; eauto.
-    * apply sel_subtrace_cons; auto.
+    * apply sel_exp_cons; auto.
   - (* Else *)
     rewrite <- H5, <- H6 in *.
     clear s'0 H7 C' H6 t H5 s0 H2 C3 H4 C0 H3 b0 H1 p0 H0.
     elim (add_sels_reduce (amend_D ps) p right (up_list p b ps (amend ps C1) (amend ps C2)) (amend ps C2) s').
     intros t1 (Ht1,Ht1').
-    exists t1, (Forget (RL_Cond p)::nil), C2, s'. repeat split; auto.
+    exists t1, (Forget _ (RL_Cond p)::nil), C2, s'. repeat split; auto.
     * econstructor. 2: apply CCT_Refl. repeat constructor; eauto.
-    * apply sel_subtrace_cons; auto.
+    * apply sel_exp_cons; auto.
   - (* Delay *)
     rewrite <- H6 in *.
     clear s'0 H7 C' H6 t0 H5 s0 H3 C3 H4 C0 H2 b0 H1 p0 H0.
@@ -751,41 +772,41 @@ induction C; intros. induction e.
     * IHElim' IHC1 (Choreography_WF_Then _ _ _ _ _ HC) HC1 tl' tl'' C'' s'' Htl' Htl'' Hsub.
       elim (add_sels_reduce (amend_D ps) p left (up_list p b ps (amend ps C1) (amend ps C2)) C'1 s').
       intros t1 (Ht1,Ht1').
-      exists (Forget (RL_Cond p)::t1++tl'), (Forget (RL_Cond p)::tl''), C'', s''.
+      exists (Forget _ (RL_Cond p)::t1++tl'), (Forget _ (RL_Cond p)::tl''), C'', s''.
       repeat split.
       econstructor; eauto. repeat constructor; auto. rewrite <- Hb; auto.
       eapply CCT_Trans; eauto.
       econstructor; eauto. repeat constructor; auto.
-      apply sel_subtrace_swap; auto.
+      apply sel_exp_swap; auto.
       rewrite <- (app_nil_r tl'').
-      apply sel_subtrace_perm' with ((Forget t :: tl') ++ t1).
-      apply sel_subtrace_app_both; auto.
+      apply sel_exp_perm' with ((Forget _ t :: tl') ++ t1).
+      apply sel_exp_app_both; auto.
       simpl. apply Permutation_cons; auto. apply Permutation_app_comm.
     * IHElim' IHC2 (Choreography_WF_Else _ _ _ _ _ HC) HC2 tl' tl'' C'' s'' Htl' Htl'' Hsub.
       elim (add_sels_reduce (amend_D ps) p right (up_list p b ps (amend ps C1) (amend ps C2)) C'2 s').
       intros t1 (Ht1,Ht1').
-      exists (Forget (RL_Cond p)::t1++tl'), (Forget (RL_Cond p)::tl''), C'', s''.
+      exists (Forget _ (RL_Cond p)::t1++tl'), (Forget _ (RL_Cond p)::tl''), C'', s''.
       repeat split.
       econstructor; eauto. constructor. apply C_Else'; eauto.
       eapply CCT_Trans; eauto.
       econstructor; eauto. repeat constructor; auto.
-      apply sel_subtrace_swap; auto.
+      apply sel_exp_swap; auto.
       rewrite <- (app_nil_r tl'').
-      apply sel_subtrace_perm' with ((Forget t :: tl') ++ t1).
-      apply sel_subtrace_app_both; auto.
+      apply sel_exp_perm' with ((Forget _ t :: tl') ++ t1).
+      apply sel_exp_app_both; auto.
       simpl. apply Permutation_cons; auto. apply Permutation_app_comm.
 + rename t0 into X. inversion H.
   - (* Local *)
     rewrite <- H6 in *.
     clear s'0 H7 C' H6 t H5 s0 H4 X0 H0 H.
-    simpl. exists nil, (Forget (RL_Call X p)::nil), (snd (Defs X)), s'.
+    simpl. exists nil, (Forget _ (RL_Call X p)::nil), (snd (Defs X)), s'.
     repeat split; repeat constructor.
     econstructor. 2: apply CCT_Refl. repeat constructor; auto.
   - (* Call *)
     rewrite <- H5 in *.
     clear s'0 H7 C' H6 t H5 s0 H4 X0 H0 H.
-    simpl. exists nil, (Forget (RL_Call X p)::nil), (RT_Call X (fst (Defs X) [\] p) (snd (Defs X))), s'.
-    repeat split; eauto. 3: apply sel_subtrace_refl.
+    simpl. exists nil, (Forget _ (RL_Call X p)::nil), (RT_Call X (fst (Defs X) [\] p) (snd (Defs X))), s'.
+    repeat split; eauto. 3: apply sel_exp_refl.
     apply CCT_Refl.
     econstructor. 2: apply CCT_Refl. repeat constructor; auto.
 + rename t0 into X. inversion H.
@@ -799,19 +820,19 @@ induction C; intros. induction e.
     repeat split; auto.
     * eapply CCT_Trans; eauto.
     * eapply CCT_Trans; eauto.
-    * apply sel_subtrace_app'; auto.
+    * apply sel_exp_app'; auto.
   - (* Enter *)
     rewrite <- H5, <- H1 in *.
     clear s'0 H7 C' H6 t H5 s0 H4 C0 H2 H X0 H0 l H1.
-    exists nil, (Forget (RL_Call X p)::nil), (RT_Call X (ps0[\]p) C), s'.
-    repeat split; eauto. 3: apply sel_subtrace_refl.
+    exists nil, (Forget _ (RL_Call X p)::nil), (RT_Call X (ps0[\]p) C), s'.
+    repeat split; eauto. 3: apply sel_exp_refl.
     apply CCT_Refl.
     econstructor. 2: apply CCT_Refl. repeat constructor; auto.
   - (* Finish *)
     rewrite <- H5, <- H1 in *.
     clear s'0 H7 C' H6 t H5 s0 H4 C0 H2 H X0 H0 l H1.
-    exists nil, (Forget (RL_Call X p)::nil), C, s'.
-    repeat split; eauto. 3: apply sel_subtrace_refl.
+    exists nil, (Forget _ (RL_Call X p)::nil), C, s'.
+    repeat split; eauto. 3: apply sel_exp_refl.
     apply CCT_Refl.
     econstructor. 2: apply CCT_Refl. repeat constructor; auto.
 + inversion H.
@@ -821,7 +842,7 @@ Lemma amend_sound_many : forall ps C s tl C' s' Xs, Program_WF _ Xs (Defs,C) ->
   (amend_D ps, amend ps C,s) --[tl]-->* (amend_D ps,C',s') ->
   exists tl' tl'' C'' s'',
   (amend_D ps,C',s') --[tl']-->* (amend_D ps, amend ps C'',s'')
-  /\ (Defs,C,s) --[tl'']-->* (Defs,C'',s'') /\ sel_subtrace tl'' (tl++tl').
+  /\ (Defs,C,s) --[tl'']-->* (Defs,C'',s'') /\ sel_exp tl'' (tl++tl').
 Proof.
 intros.
 set (n := length tl). assert (length tl <= n) as Hn; auto.
@@ -833,14 +854,14 @@ induction n; intros.
   inversion H0. rewrite <- H2 in *.
   exists nil, nil, C, s'.
   repeat split; simpl; auto. apply CCT_Refl.
-  constructor; auto; ESEr. apply sel_subtrace_refl.
+  constructor; auto; ESEr. apply sel_exp_refl.
 + case_eq tl; intros.
   1: { (* repeat... *)
     rewrite H1 in *; clear tl H1.
     inversion H0. rewrite <- H2 in *.
     exists nil, nil, C, s'.
     repeat split; simpl; auto. apply CCT_Refl.
-    constructor; auto; ESEr. apply sel_subtrace_refl.
+    constructor; auto; ESEr. apply sel_exp_refl.
   }
   rewrite H1 in *; clear tl H1.
   simpl in Hn. apply le_S_n in Hn. rename l into tl.
@@ -851,10 +872,10 @@ induction n; intros.
   intros tl0 [t0 [C0 [s0 [Htl0 [Hsub0 Htl0IF] ] ] ] ].
   induction (diamond_4b _ _ _ _ _ _ _ _ _ H2 Htl0) as [ [D C2] [tl' [tl0' [s2a [s2b [HC' [HC0 [Hs [Hperm [Hlen1 Hlen2] ] ] ] ] ] ] ] ] ].
   generalize (CCP_ToStar_Defs_stable _ _ _ _ _ _ _ _ HC'). intro H'; rewrite <- H' in *; clear D H'.
-  generalize (CCC_To_Program_WF _ _ _ _ _ _ _ (amend_Program_WF _ _ _ H) H1). intro HP''.
-  generalize (CCC_ToStar_Program_WF _ _ _ _ _ _ _ HP'' H2). intro HP'.
-  generalize (CCC_ToStar_Program_WF _ _ _ _ _ _ _ HP' HC'). intro HP2.
-  generalize (CCC_ToStar_Program_WF _ _ _ _ _ _ _ HP'' Htl0). intro HP0.
+  generalize (CCP_To_Program_WF _ _ _ _ _ _ _ (amend_Program_WF _ _ _ H) H1). intro HP''.
+  generalize (CCP_ToStar_Program_WF _ _ _ _ _ _ _ HP'' H2). intro HP'.
+  generalize (CCP_ToStar_Program_WF _ _ _ _ _ _ _ HP' HC'). intro HP2.
+  generalize (CCP_ToStar_Program_WF _ _ _ _ _ _ _ HP'' Htl0). intro HP0.
   elim (IHn C0 s0 tl0' C2 s2b); auto.
   intros tl1 [t1 [C1 [s1 [Hsub1 [Htl1 Htl1IF] ] ] ] ].
   2: etransitivity; eauto.
@@ -863,23 +884,50 @@ induction n; intros.
   - eapply CCT_Trans; eauto.
     apply CCP_ToStar_eq with s2b s1. ESEs. ESEr. auto.
   - eapply CCT_Trans; eauto.
-  - simpl. eapply sel_subtrace_trans.
-    apply sel_subtrace_app_both; eauto.
-    simpl. apply sel_subtrace_cons.
+  - simpl. eapply sel_exp_trans.
+    apply sel_exp_app_both; eauto.
+    simpl. apply sel_exp_cons.
     repeat rewrite app_assoc.
     constructor. apply Permutation_sym, Permutation_app; auto.
-  - eapply CCC_ToStar_Program_WF. 2: eauto. auto.
+  - eapply CCP_ToStar_Program_WF. 2: eauto. auto.
 Qed.
-
-(** Miscellaneous. *)
-Lemma amend_eq_End : forall ps C, amend ps C = CC.End -> C = CC.End.
-Proof. induction C; simpl; auto; discriminate. Qed.
 
 End Amend.
 
-Section Projectability.
+(** ** Additional lemmas
+These lemmas cannot be proved earlier because we made Defs a section parameter. *)
 
-(** Projectability of amendment. *)
+Section Miscellaneous.
+
+Lemma up_list_stable : forall Defs Defs' p b ps C1 C2,
+  (forall X, fst (Defs X) = fst (Defs' X)) ->
+  up_list Defs p b ps C1 C2 = up_list Defs' p b ps C1 C2.
+Proof.
+intros. induction ps; simpl; auto.
+elim (a =? p); auto.
+do 2 elim projectable_B_dec; auto.
+3: rewrite IHps; auto.
+1,2: intros; exfalso.
+all: generalize projectable_B_stable; eauto.
+Qed.
+
+(** Now we can also define amendment of a program. *)
+
+Variable ps : list Pid.
+Variable a : Ann.
+Variable P : CC.Program Sig.
+
+Definition amend_P :=
+  (amend_D (Procedures _ P) a ps, amend (Procedures _ P) a ps (Main P)).
+
+Lemma amend_P_Vars : Vars P = Vars amend_P.
+Proof. auto. Qed.
+
+End Miscellaneous.
+
+(** ** Projectability of amendment. *)
+
+Section Projectability.
 
 Lemma add_sels_proj' : forall Defs a p l ps C r, ~In r ps ->
   projectable_B Defs C r -> projectable_B Defs (add_sels a p l ps C) r.
@@ -948,36 +996,6 @@ inversion HB.
 + eexists. econstructor; eauto. all: constructor; eauto.
 Qed.
 
-Lemma bproj_stable : forall (D D':DefSet Sig) p C B,
-  (forall X, fst (D X) = fst (D' X)) ->
-  [[D,C | p]] == B -> [[D',C | p]] == B.
-Proof.
-intros. induction H0; auto.
-all: try constructor; auto.
-2,3: rewrite <- H; auto.
-apply bproj_Cond' with B1 B2; auto.
-Qed.
-
-Lemma projectable_B_stable : forall (D D':DefSet Sig) p C,
-  (forall X, fst (D X) = fst (D' X)) ->
-  projectable_B D p C -> projectable_B D' p C.
-Proof.
-intros. induction H0 as [B HB].
-exists B. apply bproj_stable with D; auto.
-Qed.
-
-Lemma up_list_stable : forall Defs Defs' p b ps C1 C2,
-  (forall X, fst (Defs X) = fst (Defs' X)) ->
-  up_list Defs p b ps C1 C2 = up_list Defs' p b ps C1 C2.
-Proof.
-intros. induction ps; simpl; auto.
-elim (a =? p); auto.
-do 2 elim projectable_B_dec; auto.
-3: rewrite IHps; auto.
-1,2: intros; exfalso.
-all: generalize projectable_B_stable; eauto.
-Qed.
-
 Lemma amend_projectable_B : forall Defs a r ps C,
   In r ps -> projectable_B (amend_D Defs a ps) (amend Defs a ps C) r.
 Proof.
@@ -1018,401 +1036,8 @@ Qed.
 
 End Projectability.
 
-Local Ltac sup := rewrite set_union_iff; auto.
-
-Lemma add_sels_CCC_pn_C : forall ps a p l C f,
-  CCC_pn C f [C] CCC_pn (add_sels a p l ps C) f.
-Proof. red; intros. induction ps; simpl; auto. sup. Qed.
-
-Lemma add_sels_CCC_pn_ps : forall ps a p l C f,
-  ps [C] CCC_pn (add_sels a p l ps C) f.
-Proof.
-red; intros.
-induction ps, H.
-all: simpl; sup. rewrite H; simpl; auto.
-Qed.
-
-Lemma add_sels_CCC_pn : forall ps a p l C f,
-  CCC_pn (add_sels a p l ps C) f [C] (p :: CCC_pn C f [U] ps).
-Proof.
-intros; induction ps; simpl; auto.
-red; simpl; auto.
-red; red in IHps; intros.
-simpl; rewrite set_add_iff.
-rewrite set_union_iff in H.
-induction H as [ [H | [H | H] ] | H]; auto.
-inversion H. elim (IHps z); auto.
-Qed.
-
-Lemma amend_CCC_pn_C : forall ps a f Defs C,
-  CCC_pn C f [C] CCC_pn (amend Defs a ps C) f.
-Proof.
-red; intros. induction C; simpl; auto.
-all: sup.
-+ induction e; simpl in H; rewrite set_union_iff in H; tauto.
-+ simpl in H. repeat rewrite set_union_iff in H.
-  induction H as [ [H | H] | H]; sup.
-  1: left; right. 2: right.
-  all: apply add_sels_CCC_pn_C; auto.
-+ simpl in H. rewrite set_union_iff in H; tauto.
-Qed.
-
-Lemma up_list_incl : forall Defs p b ps C1 C2, up_list Defs p b ps C1 C2 [C] ps.
-Proof.
-red; intros. induction ps; simpl; auto.
-revert H; simpl. elim eqb; auto.
-elim projectable_B_dec; auto.
-simpl; intros. inversion_clear H; auto.
-Qed.
-
-Lemma up_list_incl_C : forall Defs p b ps C1 C2,
-  up_list Defs p b ps C1 C2 [C] (CCC_pn C1 (Names Defs) [U] CCC_pn C2 (Names Defs)).
-Proof.
-red; intros. induction ps; simpl; auto. inversion H.
-generalize H; simpl.
-case_eq (a =? p); intro; auto.
-elim projectable_B_dec; intros; auto.
-elim (In_dec (@eq_dec Pid) z (up_list Defs p b ps C1 C2)); auto.
-intro. inversion_clear H1; auto.
-rewrite H2 in *; clear a H2.
-elim (In_dec (@eq_dec Pid) z (CCC_pn C1 (Names Defs) [U] CCC_pn C2 (Names Defs))); auto.
-intro. elim b0.
-exists (End _). apply bproj_not_In; auto.
-simpl. repeat sup.
-intro; apply b2. repeat sup. 
-induction H1 as [ [H1 | H1] | H1]; auto.
-rewrite eqb_neq in H0. simpl in H1.
-inversion_clear H1; exfalso; auto.
-Qed.
-
-Lemma amend_CCC_pn_incl : forall ps a Defs C,
-  CCC_pn (amend Defs a ps C) (Names Defs) [C] CCC_pn C (Names Defs).
-Proof.
-red; intros. induction C. induction e.
-all: simpl; auto.
-all: simpl in H; repeat rewrite set_union_iff in H.
-all: inversion_clear H; repeat sup.
-inversion_clear H0; auto.
-2: rename H0 into H.
-all: apply add_sels_CCC_pn in H.
-all: inversion_clear H. 1,3: rewrite H0; simpl; auto.
-all: rewrite set_union_iff in H0; inversion_clear H0; auto.
-all: apply up_list_incl_C in H; rewrite set_union_iff in H; tauto.
-Qed.
-
-Variable ps : list Pid.
-Variable a : Ann.
-Variable P : CC.Program Sig.
-
-Definition amend_P :=
-  (amend_D (Procedures _ P) a ps, amend (Procedures _ P) a ps (Main P)).
-
-Lemma amend_P_Vars : Vars P = Vars amend_P.
-Proof. auto. Qed.
-
 End Amendment.
 
 Arguments amend [Sig].
 Arguments amend_D [Sig].
 Arguments amend_P [Sig].
-
-Require Export EPPTheorem.
-Require Export Implementation.
-
-Section TuringRevisited.
-
-Theorem amended_encoding_WF : forall n (f:PRFunction n),
-  CCP_WF (amend_P (all_pids (n+Pi f)) eps (Encoding' f)).
-Proof.
-intros.
-induction (Encoding'_WF f) as [Hann [Xs HWF] ].
-split.
-+ red; simpl; intros. rewrite <- amend_P_Vars.
-  clear Xs HWF.
-  red; intros. apply Hann.
-  induction (Encoding' f) as (D,C).
-  unfold Procs, Procedures, amend_P in H. simpl in H.
-  generalize amend_CCC_pn_incl; intro.
-  red in H0. eauto.
-+ exists Xs. apply amend_Program_WF; auto.
-Qed.
-
-Lemma amend_implements : forall n (f:PRFunction n) ps q P ps' a Xs,
-  Program_WF _ Xs P -> implements P f ps q -> implements (amend_P ps' a P) f ps q.
-Proof.
-red; intros. rename H into HP, H1 into Hps.
-induction (H0 xs s) as [Hconv Hdiv]; auto.
-induction P as (Defs,C).
-split; intros.
-1: induction (Hconv y) as [Hto Hfrom]; clear Hconv Hdiv.
-2: induction Hdiv as [Hto Hfrom]; clear Hconv.
-all: split; intros.
-+ (* function converges *)
-  specialize (Hto H); clear Hfrom.
-  induction Hto as [s' [ts [P' [Hred [Hs' HP'] ] ] ] ].
-  induction P' as (Defs',C').
-  generalize (CCP_ToStar_Defs_stable _ _ _ _ _ _ _ _ Hred) as HDefs; intros.
-  rewrite <- HDefs in *; clear Defs' HDefs. simpl in *.
-  rewrite HP' in *; clear C' HP'.
-  apply amend_complete_many with (a:=a) (ps:=ps') (Xs:=Xs) in Hred; auto.
-  induction Hred as (tl',(tl'',(C'',(s'',(Hsub,(Htl',Htl'')))))).
-  generalize (CCP_ToStar_End _ _ _ _ _ _ Htl'); intro H'.
-  induction H' as [H1 H2]; auto. rewrite H1 in *; clear H1 tl'.
-  inversion Htl'. rewrite <- H3 in *; clear s'0 H6 C'' H3 s0 H4 P H1 H5.
-  exists s'', tl''; eexists. repeat split; eauto.
-  rewrite <- H2; auto.
-+ (* choreography terminates *)
-  apply Hfrom; clear Hto Hfrom.
-  induction H as (s',(ts,(P',(Hts,(Hs',HP'))))).
-  induction P' as (Defs',C'). simpl in *; rewrite HP' in *; clear C' HP'.
-  rewrite <- (CCP_ToStar_Defs_stable _ _ _ _ _ _ _ _ Hts) in Hts; clear Defs'.
-  apply amend_sound_many with (Xs:=Xs) in Hts; auto.
-  induction Hts as (tl',(tl'',(C'',(s'',(Htl',(Htl'',Hsub)))))).
-  generalize (CCP_ToStar_End _ _ _ _ _ _ Htl'); intro H'.
-  induction H' as [H1 H2]; auto. rewrite H1 in *; clear H1 tl'.
-  inversion Htl'. symmetry in H1. rewrite (amend_eq_End _ _ _ _ _ H1) in *.
-  clear s'0 H5 C'' H1 s0 H3 P H H4.
-  exists s'', tl'', (Defs,End). repeat split; auto.
-  rewrite <- H2; auto.
-+ (* function diverges *)
-  specialize (Hto H); clear H Hfrom.
-  induction P' as (Defs',C').
-  generalize (CCP_ToStar_Defs_stable _ _ _ _ _ _ _ _ H1) as HDefs; intros.
-  rewrite <- HDefs in *; clear Defs' HDefs. simpl in *.
-  apply amend_sound_many with (Xs:=Xs) in H1; auto.
-  induction H1 as (tl',(tl'',(C'',(s'',(Htl',(Htl'',Hsub)))))).
-  simpl in Htl''. specialize (Hto _ _ _ Htl'').
-  intro. apply Hto; simpl.
-  rewrite H in *; clear C' H. simpl in *.
-  generalize (CCP_ToStar_End _ _ _ _ _ _ Htl'); intro H'.
-  induction H' as [H1 H2]; auto. rewrite H1 in *; clear H1 tl'.
-  inversion Htl'. symmetry in H1. apply (amend_eq_End _ _ _ _ _ H1).
-+ (* choreography diverges *)
-  apply Hfrom; clear Hto Hfrom; intros.
-  induction P' as (Defs',C').
-  generalize (CCP_ToStar_Defs_stable _ _ _ _ _ _ _ _ H1) as HDefs; intros.
-  rewrite <- HDefs in *; clear Defs' HDefs. simpl in *.
-  apply amend_complete_many with (a:=a) (ps:=ps') (Xs:=Xs) in H1; auto.
-  induction H1 as (tl',(tl'',(C'',(s'',(Hsub,(Htl',Htl'')))))).
-  intro HC'. rewrite HC' in *; clear C' HC'.
-  generalize (CCP_ToStar_End _ _ _ _ _ _ Htl'); intro H'.
-  induction H' as [H1 H2]; auto. rewrite H1 in *; clear H1 tl'.
-  inversion Htl'. rewrite <- H3 in *; clear s'0 H6 C'' H3 s0 H4 P H1 H5.
-  apply (H _ _ _ Htl''); auto.
-Qed.
-
-Theorem amended_encoding_sound : forall n (f:PRFunction n),
-  implements (amend_P (all_pids (n+Pi f)) eps (Encoding' f)) f (vec_1_to_n n) 0.
-Proof.
-intros.
-induction (Encoding'_WF f) as [Hann [Xs HP] ].
-apply amend_implements with Xs; auto.
-apply encoding_sound.
-Qed.
-
-Lemma vmax_vec_1_to_n : forall n, vmax (vec_1_to_n n) = n.
-Proof.
-intro. unfold vec_1_to_n.
-destruct n; auto.
-rewrite vec_k_to_n_vmax.
-apply Nat.add_sub.
-auto with arith.
-Qed.
-
-Theorem amended_encoding_projectable : forall n (f:PRFunction n),
-  projectable _ (RecVarList (Gamma f)) (all_pids (n+Pi f)) (amend_P (all_pids (n+Pi f)) eps (Encoding' f)).
-Proof.
-intros.
-induction (Encoding'_WF f) as [Hann [Xs HWF] ].
-repeat split.
-+ apply amend_projectable_C.
-+ red. rewrite List.Forall_forall; intros.
-  unfold Procedures, amend_P.
-  set (P := Encoding' f). assert (P = Encoding' f); auto.
-  clearbody P. induction P as (D,C). simpl.
-  red; rewrite List.Forall_forall; intros.
-  apply amend_projectable_B.
-  unfold Encoding', Encoding in H0.
-  change D with (fst (D,C)) in H1. rewrite H0 in H1. simpl in H1.
-  rewrite vmax_vec_1_to_n in H1; auto.
-+ unfold amend_P; simpl. tauto.
-+ set (P := Encoding' f). assert (P = Encoding' f); auto.
-  clearbody P. induction P as (D,C). simpl.
-  unfold Encoding', Encoding in H.
-  intros. change D with (fst (D,C)) in H1.
-  rewrite H in H1. simpl in H1.
-  rewrite vmax_vec_1_to_n in H1; auto.
-+ set (P := Encoding' f). assert (P = Encoding' f); auto.
-  clearbody P. induction P as (D,C). simpl; intros.
-  specialize (Hann X p). rewrite <- H in Hann.
-  unfold Encoding', Encoding in H.
-  intros. apply CCC_pn_mon with (Y:=Names D) in H1.
-  2: simpl; tauto.
-  apply amend_CCC_pn_incl in H1.
-  apply Hann in H1.
-  change D with (fst (D,C)) in H1.
-  rewrite H in H1. simpl in H1.
-  rewrite vmax_vec_1_to_n in H1; auto.
-Qed.
-
-Theorem amended_encoding_Projectable : forall n (f:PRFunction n),
-  Projectable _ (amend_P (all_pids (n+Pi f)) eps (Encoding' f)).
-Proof.
-intros.
-induction (Encoding'_WF f) as [Hann [Xs HWF] ].
-(* this should be simplifiable *)
-exists Xs, (all_pids (n+Pi f)); split. repeat split.
-+ apply amend_projectable_C.
-+ red. rewrite List.Forall_forall; intros.
-  unfold Procedures, amend_P.
-  set (P := Encoding' f). assert (P = Encoding' f); auto.
-  clearbody P. induction P as (D,C). simpl.
-  red; rewrite List.Forall_forall; intros.
-  apply amend_projectable_B.
-  unfold Encoding', Encoding in H0.
-  change D with (fst (D,C)) in H1. rewrite H0 in H1. simpl in H1.
-  rewrite vmax_vec_1_to_n in H1; auto.
-+ unfold amend_P; simpl. tauto.
-+ set (P := Encoding' f). assert (P = Encoding' f); auto.
-  clearbody P. induction P as (D,C). simpl.
-  unfold Encoding', Encoding in H.
-  intros. change D with (fst (D,C)) in H1.
-  rewrite H in H1. simpl in H1.
-  rewrite vmax_vec_1_to_n in H1; auto.
-+ set (P := Encoding' f). assert (P = Encoding' f); auto.
-  clearbody P. induction P as (D,C). simpl; intros.
-  specialize (Hann X p). rewrite <- H in Hann.
-  unfold Encoding', Encoding in H.
-  intros. apply CCC_pn_mon with (Y:=Names D) in H1.
-  2: simpl; tauto.
-  apply amend_CCC_pn_incl in H1.
-  apply Hann in H1.
-  change D with (fst (D,C)) in H1.
-  rewrite H in H1. simpl in H1.
-  rewrite vmax_vec_1_to_n in H1; auto.
-+ apply amend_Program_WF; auto.
-Qed.
-
-End TuringRevisited.
-
-Section SP_Turing.
-
-Open Scope SP_scope.
-
-Definition SP_implements (P:SP.Program (Sig' IS)) {n} (f:PRFunction n) (ps:t Pid n) (q:Pid) :=
-  forall (xs:t nat n) s, (forall Hi, s (ps[@Hi]) xx = xs[@Hi]) ->
-  (forall y, converges f xs y <-> exists s' ts P',
-      (P,s) --[ts]-->* (P',s') /\ s' q xx = y /\ Net P' (==) EmptyNet _) /\
-  (diverges f xs <-> forall s' ts P', (P,s) --[ts]-->* (P',s') -> ~(Net P' (==) EmptyNet _)).
-
-Definition Encode_Net {n} f := epp _ _ _ (amended_encoding_projectable n f).
-
-Lemma epp_implements : forall n (f:PRFunction n) P Xs ps q ps',
-  Program_WF _ Xs P -> well_ann _ P -> forall (HP:projectable _ Xs ps' P),
-  (forall p, List.In p ps' -> str_proj (Procedures _ P) (Main P) p) ->
-  (forall p, List.In p (CCC_pn (Main P) (Vars P)) -> List.In p ps') ->
-  (forall p X, List.In X Xs -> List.In p (Vars P X) -> List.In p ps') ->
-  implements P f ps q -> SP_implements (epp Xs ps' P HP) f ps q.
-Proof.
-intros.
-rename H0 into Hann, H1 into Hsp, H2 into Hpn, H3 into Hin, H4 into Himpl.
-red; intros.
-induction (Himpl _ _ H0) as [Hconv Hdiv]; clear H0.
-repeat split.
-+ (* f converges *)
-  intros. elim (Hconv y); intros. specialize (H1 H0).
-  clear Hconv Hdiv H0 H2.
-  induction H1 as [s' [ts [P' [Hts [Hs' HP'] ] ] ] ].
-  induction P as (D,C), P' as (D',C').
-  generalize (CCP_ToStar_Defs_stable _ _ _ _ _ _ _ _ Hts); intro HD.
-  simpl in HP'. rewrite <- HD, HP' in *; clear C' D' HD HP'.
-  apply EPP_Complete' with (HP:=HP) in Hts; auto.
-  induction Hts as [N [tl' [Htl' HN] ] ].
-  exists s', tl', N. repeat split; auto.
-  assert (projectable_C D End ps').
-  1:{ red; rewrite List.Forall_forall; intros.
-      exists (SP.End _); constructor.
-  }
-  assert (projectable IS Xs ps' (D,End)).
-  1: { elim HP. intros HC (HD,(H1,(H2,H3))).
-       repeat split; auto. simpl; tauto.
-  }
-  specialize (HN H1).
-  generalize (epp_C_char _ _ _ _ _ H1 H0); intros.
-  intro. specialize (HN p). rewrite H2 in HN.
-  rewrite epp_C_End in HN. inversion HN; auto.
-+ (* N terminates *)
-  intros. apply (Hconv y); intros. clear Hconv Hdiv.
-  induction H0 as [s' [ts [P' [Hts [Hs' HP'] ] ] ] ].
-  apply EPP_Sound' in Hts; auto.
-  induction Hts as [P'' [ts' [Htl' HN] ] ].
-  exists s', ts', P''; repeat split; auto.
-  apply CCC_ToStar_projectable with (s:=s) (tl:=ts') (P':=P'') (s':=s') in HP; auto.
-  specialize (HN HP).
-  apply epp_EmptyNet' with (HP:=HP) (N:=Net P'); auto.
-  apply (CCC_ToStar_Program_WF _ _ _ _ _ _ _ H Htl').
-+ (* f diverges *)
-  induction Hdiv; intros. specialize (H0 H2). clear Hconv H1 H2.
-  apply EPP_Sound' in H3.
-  induction H3 as [P'' [ts' [Htl' HN] ] ].
-  intro. eapply H0; eauto. all: auto.
-  apply CCC_ToStar_projectable with (s:=s) (tl:=ts') (P':=P'') (s':=s') in HP; auto.
-  apply epp_EmptyNet' with (HP:=HP) (N:=Net P'); auto.
-  apply (CCC_ToStar_Program_WF _ _ _ _ _ _ _ H Htl').
-+ (* N loops *)
-  intros. apply Hdiv; intros. clear Hconv Hdiv.
-  induction P as (D,C), P' as (D',C').
-  generalize (CCP_ToStar_Defs_stable _ _ _ _ _ _ _ _ H1); intros HD HC'.
-  simpl in HC'. rewrite HC', <- HD in *; clear D' C' HD HC'.
-  apply EPP_Complete' with (HP:=HP) in H1; auto.
-  induction H1 as [N [tl' [Htl' HN] ] ].
-  eapply H0; eauto.
-  assert (projectable_C D End ps').
-  1:{ red; rewrite List.Forall_forall; intros.
-      exists (SP.End _); constructor.
-  }
-  assert (projectable IS Xs ps' (D,End)).
-  1: { elim HP. intros HC (HD,(H2,(H3,H4))).
-       repeat split; auto. simpl; tauto.
-  }
-  specialize (HN H2).
-  generalize (epp_C_char _ _ _ _ _ H2 H1); intros.
-  intro. specialize (HN p). rewrite H3 in HN.
-  rewrite epp_C_End in HN. inversion HN; auto.
-Qed.
-
-Theorem encode_Net_sound : forall n (f:PRFunction n),
-  SP_implements (Encode_Net f) f (vec_1_to_n n) 0.
-Proof.
-intros.
-induction (amended_encoding_WF n f) as [Hann [Xs HXs] ].
-apply epp_implements; auto.
-+ apply amend_Program_WF; auto.
-  split. apply Encoding_Main_WF.
-  split. apply Encoding_Main_within_Xs; apply RecVarList_In; auto with arith.
-  split. simpl; auto.
-  split.
-  1: { apply Encoding_rec_WF; intros; auto.
-       intro. elim (in_vec_k_to_n _ H0); intros.
-       inversion H1.
-    2: auto with arith.
-    elim (in_vec_k_to_n _ H0); intros.
-    rewrite vmax_vec_1_to_n; auto.
-  }
-  split. apply Encoding_rec_initial.
-  split. apply Encoding_Procs_Vars_not_nil.
-  change (Gamma f) with (0 + Gamma f).
-  apply Encoding_rec_within_Xs; simpl; auto.
-+ intros. apply HXs.
-+ intros. simpl in H.
-  rewrite <- amend_P_Vars in H.
-  unfold Vars, Encoding', Procedures in H.
-  simpl in H.
-  rewrite vmax_vec_1_to_n in H; auto.
-+ intros. unfold Vars, Encoding', Procedures in H0.
-  simpl in H0.
-  rewrite vmax_vec_1_to_n in H0; auto.
-+ apply amended_encoding_sound.
-Qed.
-
-End SP_Turing.
